Refactor FlatThread

src/FlatThread.v
@@ -32,57 +32,54 @@ Import Word.Notations.
 Require Import Types Utils.
 Require Import  Decision.
 
-Module Make (Arc : ArcSig) : ThreadSig Arc.
-  Export Arc.
-  Existing Instance showable_ast.
-  Existing Instance decision_reg_eq.
-  Existing Instance showable_regE.
-
-  Variant _E : Type -> Type :=
-  | ThEFetchAndDecodeOrRestart : _E (list instruction_id * ast)
-  | ThEFinishIns : _E unit
-  | ThERegAccess : forall A, regE A -> _E A
-  (** Load events *)
-  | ThEInitMemLoadOps : mem_slc -> _E (list mem_read_id)
-  (* [ThESatMemLoadOpForwarding] returns a bool that indicates if the read
-     was fully satisfied, and a list of iids that should be restarted. *)
-  | ThESatMemLoadOpForwarding : mem_read_id -> _E (bool * list instruction_id)
-  (* [ThESatMemLoadOpStorage] returns a list of iids that should be restarted. *)
-  | ThESatMemLoadOpStorage : mem_read_id -> _E (list instruction_id)
-  | ThECompleteLoadOps : _E mem_slc_val
-  (** Store events *)
-  | ThEInitMemStoreOpFps : mem_slc -> _E unit
-  | ThEInstaMemStoreOpVals : mem_slc_val -> _E unit
-  | ThECommitStoreInstruction : _E (list mem_write_id)
-  (* [ThEPropagateStoreOp] returns a list of iids that should be restarted. *)
-  | ThEPropagateStoreOp : mem_write_id -> _E (list instruction_id)
-  | ThECompleteStoreOps : _E unit.
-  (* Workaround: parameter can't be instantiated by an inductive type *)
-  Definition E := _E.
-
-  Instance showable_E : forall A, Showable (E A) :=
-    { show := fun e =>
-                match e with
-                | ThEFetchAndDecodeOrRestart => "ThEFetchAndDecodeOrRestart"
-                | ThEFinishIns => "ThEFinishIns"
-                | ThERegAccess _ e => "ThERegAccess (" ++ show e ++ ")"
-                (** Load events *)
-                | ThEInitMemLoadOps slc => "ThEInitMemLoadOps " ++ show slc
-                | ThESatMemLoadOpForwarding rid => "ThESatMemLoadOpForwarding " ++ show rid
-                | ThESatMemLoadOpStorage rid => "ThESatMemLoadOpStorage " ++ show rid
-                | ThECompleteLoadOps => "ThECompleteLoadOps"
-                (** Store events *)
-                | ThEInitMemStoreOpFps slc => "ThEInitMemStoreOpFps " ++ show slc
-                | ThEInstaMemStoreOpVals val => "ThEInstaMemStoreOpVals " ++ show val
-                | ThECommitStoreInstruction => "ThECommitStoreInstruction"
-                | ThEPropagateStoreOp wid => "ThEPropagateStoreOp " ++ show wid
-                | ThECompleteStoreOps => "ThECompleteStoreOps"
-                end%string
-    }.
+Module Base (Arc : ArcSig).
+  Import Arc.
 
   Section Denote.
+    Variant _E : Type -> Type :=
+    | ThEFetchAndDecodeOrRestart : _E (list instruction_id * ast)
+    | ThEFinishIns : _E unit
+    | ThERegAccess : forall A, regE A -> _E A
+    (** Load events *)
+    | ThEInitMemLoadOps : mem_slc -> _E (list mem_read_id)
+    (* [ThESatMemLoadOpForwarding] returns a bool that indicates if the read
+     was fully satisfied, and a list of iids that should be restarted. *)
+    | ThESatMemLoadOpForwarding : mem_read_id -> _E (bool * list instruction_id)
+    (* [ThESatMemLoadOpStorage] returns a list of iids that should be restarted. *)
+    | ThESatMemLoadOpStorage : mem_read_id -> _E (list instruction_id)
+    | ThECompleteLoadOps : _E mem_slc_val
+    (** Store events *)
+    | ThEInitMemStoreOpFps : mem_slc -> _E unit
+    | ThEInstaMemStoreOpVals : mem_slc_val -> _E unit
+    | ThECommitStoreInstruction : _E (list mem_write_id)
+    (* [ThEPropagateStoreOp] returns a list of iids that should be restarted. *)
+    | ThEPropagateStoreOp : mem_write_id -> _E (list instruction_id)
+    | ThECompleteStoreOps : _E unit.
+    (* Workaround: parameter can't be instantiated by an inductive type *)
+    Definition E := _E.
+
+    #[global] Instance showable_E : forall A, Showable (E A) :=
+      { show := fun e =>
+                  match e with
+                  | ThEFetchAndDecodeOrRestart => "ThEFetchAndDecodeOrRestart"
+                  | ThEFinishIns => "ThEFinishIns"
+                  | ThERegAccess _ e => "ThERegAccess (" ++ show e ++ ")"
+                  (** Load events *)
+                  | ThEInitMemLoadOps slc => "ThEInitMemLoadOps " ++ show slc
+                  | ThESatMemLoadOpForwarding rid => "ThESatMemLoadOpForwarding " ++ show rid
+                  | ThESatMemLoadOpStorage rid => "ThESatMemLoadOpStorage " ++ show rid
+                  | ThECompleteLoadOps => "ThECompleteLoadOps"
+                  (** Store events *)
+                  | ThEInitMemStoreOpFps slc => "ThEInitMemStoreOpFps " ++ show slc
+                  | ThEInstaMemStoreOpVals val => "ThEInstaMemStoreOpVals " ++ show val
+                  | ThECommitStoreInstruction => "ThECommitStoreInstruction"
+                  | ThEPropagateStoreOp wid => "ThEPropagateStoreOp " ++ show wid
+                  | ThECompleteStoreOps => "ThECompleteStoreOps"
+                  end%string
+      }.
+
     Definition lift_regE {F} `{E -< F}
-    : regE ~> itree F :=
+      : regE ~> itree F :=
       fun _ e => trigger (ThERegAccess _ e).
 
     Definition denote_spawns  {F} `{schedulerE instruction_id -< F}
@@ -91,15 +88,15 @@ Module Make (Arc : ArcSig) : ThreadSig Arc.
         List.fold_left
           (fun it iid => Vis (subevent _ (Spawn iid)) (fun 'tt => it))
           iids (Ret tt).
-        (* The fold above can also be implemented as below. I'm not sure which
+    (* The fold above can also be implemented as below. I'm not sure which
            way is better. The implementation above has less [Tau]s, and
            therefore less nondet interleaving, but that is not a big factor. *)
-        (* ITree.iter (fun iids => *)
-        (*               match iids with *)
-        (*               | [] => ret (inr tt) *)
-        (*               | iid::iids => 'tt <- trigger (Spawn iid) *)
-        (*                            ;; ret (inl iids) *)
-        (*               end) iids. *)
+    (* ITree.iter (fun iids => *)
+    (*               match iids with *)
+    (*               | [] => ret (inr tt) *)
+    (*               | iid::iids => 'tt <- trigger (Spawn iid) *)
+    (*                            ;; ret (inl iids) *)
+    (*               end) iids. *)
 
     Definition denote_restarts {F} `{schedulerE instruction_id -< F}
       : ktree F (list instruction_id) unit :=
@@ -127,15 +124,15 @@ Module Make (Arc : ArcSig) : ThreadSig Arc.
                                          (restarts <- trigger (ThESatMemLoadOpStorage rid)
                                           ;; ret (true, restarts))] in
                             read <- nondet reads
-                         ;; read <- try_unwrap_option read
-                                                     "lift_mem_read: nondet out of range"
-                         ;; is_sat <- exclusive_block
-                                       ('(is_sat, restarts) <- read
-                                        ;; 'tt <- denote_restarts restarts
-                                        ;; ret is_sat)
-                         ;; ret (inl (if (is_sat : bool) then
-                                        List.remove decision_mem_read_id_eq rid rids
-                                      else rids))
+                            ;; read <- try_unwrap_option read
+                                                        "lift_mem_read: nondet out of range"
+                            ;; is_sat <- exclusive_block
+                                          ('(is_sat, restarts) <- read
+                                           ;; 'tt <- denote_restarts restarts
+                                           ;; ret is_sat)
+                            ;; ret (inl (if (is_sat : bool) then
+                                           List.remove decision_mem_read_id_eq rid rids
+                                         else rids))
                        end) rids.
 
     Definition lift_mem_write_fp {F} `{E -< F}
@@ -206,12 +203,12 @@ Module Make (Arc : ArcSig) : ThreadSig Arc.
         resum_it _ (wrap_event_in_it E iid _ it).
 
     Definition is_eager_event {A T} : (wrapE E T
-                                     +' chooseE mem_read_id
-                                     +' chooseE mem_write_id
-                                     +' chooseE nat
-                                     +' exceptE error
-                                     +' debugE) A
-                                    -> bool :=
+                                       +' chooseE mem_read_id
+                                       +' chooseE mem_write_id
+                                       +' chooseE nat
+                                       +' exceptE error
+                                       +' debugE) A
+                                      -> bool :=
       fun e =>
         match e with
         | inl1 (Wrap e _) => (* wrapE E T *)
@@ -289,7 +286,14 @@ Module Make (Arc : ArcSig) : ThreadSig Arc.
                               None).
   End Denote.
 
+  (*****************************************************************************)
+
+  Existing Instance decision_reg_eq.
+
   Section State.
+    Existing Instance showable_ast.
+    Existing Instance showable_regE.
+
     Record reg_read_state :=
       mk_reg_read_state { rrs_slc : reg_slc;
                           rrs_feeding_addr : bool;
@@ -334,7 +338,7 @@ Module Make (Arc : ArcSig) : ThreadSig Arc.
                            rs_unsat_slcs : list (list mem_slc);
                            rs_reads_from : list mem_reads_from }.
 
-    Instance eta_mem_reads_state : Settable _ :=
+    #[global] Instance eta_mem_reads_state : Settable _ :=
       settable! mk_mem_reads_state <rs_footprint; rs_reads; rs_unsat_slcs; rs_reads_from>.
 
     Instance showable_mem_reads_state : Showable mem_reads_state :=
@@ -347,7 +351,7 @@ Module Make (Arc : ArcSig) : ThreadSig Arc.
                             ws_writes : list mem_write;
                             ws_has_propagated : list bool }.
 
-    Instance eta_mem_writes_state : Settable _ :=
+    #[global] Instance eta_mem_writes_state : Settable _ :=
       settable! mk_mem_writes_state <ws_footprint; ws_writes; ws_has_propagated>.
 
     Instance showable_mem_writes_state : Showable mem_writes_state :=
@@ -370,7 +374,7 @@ Module Make (Arc : ArcSig) : ThreadSig Arc.
 
           ins_finished : bool }.
 
-    Instance eta_decoded_instruction_state : Settable _ :=
+    #[global] Instance eta_decoded_instruction_state : Settable _ :=
       settable! mk_decoded_instruction_state <ins_id; ins_loc; ins_ast; ins_reg_reads; ins_reg_writes; ins_mem_reads; ins_mem_writes; ins_finished>.
 
     Local Open Scope string_scope.
@@ -378,26 +382,26 @@ Module Make (Arc : ArcSig) : ThreadSig Arc.
       { show :=
           fun i =>
             show i.(ins_id) ++ ":[" ++ show i.(ins_loc) ++ "] " ++
-              ("'" ++ show i.(ins_ast) ++ "' " ++
-                                       (if i.(ins_finished) then "(finished)"
-                                        else "(in-flight)") ++ newline ++
-             match i.(ins_reg_reads) with
-             | [] => ""
-             | _ => "  reg reads: " ++ show i.(ins_reg_reads) ++ newline
-             end ++
-             match i.(ins_reg_writes) with
-             | [] => ""
-             | _ => "  reg writes: " ++ show i.(ins_reg_writes) ++ newline
-             end ++
-             match i.(ins_mem_reads) with
-             | Some rs => "  mem reads: " ++ show rs ++ newline
-             | None => ""
-             end ++
-             match i.(ins_mem_writes) with
-             | Some ws => "  mem writes: " ++ show ws ++ newline
-             | None => ""
-             end
-            )%string
+                                                        ("'" ++ show i.(ins_ast) ++ "' " ++
+                                                                                 (if i.(ins_finished) then "(finished)"
+                                                                                  else "(in-flight)") ++ newline ++
+                                                                                 match i.(ins_reg_reads) with
+                                                                                 | [] => ""
+                                                                                 | _ => "  reg reads: " ++ show i.(ins_reg_reads) ++ newline
+                                                                                 end ++
+                                                                                 match i.(ins_reg_writes) with
+                                                                                 | [] => ""
+                                                                                 | _ => "  reg writes: " ++ show i.(ins_reg_writes) ++ newline
+                                                                                 end ++
+                                                                                 match i.(ins_mem_reads) with
+                                                                                 | Some rs => "  mem reads: " ++ show rs ++ newline
+                                                                                 | None => ""
+                                                                                 end ++
+                                                                                 match i.(ins_mem_writes) with
+                                                                                 | Some ws => "  mem writes: " ++ show ws ++ newline
+                                                                                 | None => ""
+                                                                                 end
+                                                        )%string
       }.
     Close Scope string_scope.
 
@@ -420,7 +424,7 @@ Module Make (Arc : ArcSig) : ThreadSig Arc.
          ins_mem_writes := None;
          ins_finished := false |}.
 
-    Notation ins_tree := (tree decoded_instruction_state
+    Definition ins_tree := (tree decoded_instruction_state
                                (tree (instruction_id * mem_loc) unit))%type.
     Record _state :=
       mk_state { next_iid : instruction_id;
@@ -428,7 +432,7 @@ Module Make (Arc : ArcSig) : ThreadSig Arc.
     (* Workaround: parameter can't be instantiated by an inductive type *)
     Definition state := _state.
 
-    Instance eta_state : Settable _ :=
+    #[global] Instance eta_state : Settable _ :=
       settable! mk_state <next_iid; instruction_tree>.
 
     Local Open Scope string_scope.
@@ -452,8 +456,8 @@ Module Make (Arc : ArcSig) : ThreadSig Arc.
                 | TNode i [t] => (show i.(ins_id)) ++ "," ++ show_dec_tree t
                 | TNode i ts =>
                   (show i.(ins_id)) ++ "["
-                             ++ String.concat ";" (List.map show_dec_tree ts)
-                             ++ "]"
+                                    ++ String.concat ";" (List.map show_dec_tree ts)
+                                    ++ "]"
                 end in
             let show_ins i :=
                 match i with
@@ -468,551 +472,668 @@ Module Make (Arc : ArcSig) : ThreadSig Arc.
                   String.concat "" (List.map show_ins (tree_to_list_preorder t))
                 end in
             "Instruction tree: " ++ newline ++
-            "  " ++ (show_dec_tree s.(instruction_tree)) ++ newline ++
-            "Instructions:" ++ newline ++
-            String.concat "" (List.map show_ins (tree_to_list_preorder s.(instruction_tree)))
+                                 "  " ++ (show_dec_tree s.(instruction_tree)) ++ newline ++
+                                 "Instructions:" ++ newline ++
+                                 String.concat "" (List.map show_ins (tree_to_list_preorder s.(instruction_tree)))
       }.
     Close Scope string_scope.
+  End State.
+End Base.
 
-    Definition initial_state '((InstructionID iid) : instruction_id) (loc : mem_loc)
-      : state :=
-      {| next_iid := InstructionID (iid + 1);
-         instruction_tree := TLeaf (TNode (InstructionID iid, loc) []) |}.
+(******************************************************************************)
 
-    Section RegisterRead.
-      Local Instance slice_id_rsv : Slice (instruction_id * nat * reg_slc_val) :=
-        { start := fun '(_, _, s) => Utils.start s;
-          size := fun '(_, _, s) => Utils.size s;
-          sub_slice := fun '(id, s) start size =>
-                         match sub_slice s start size with
-                         | Some s' => Some (id, s')
-                         | None => None
-                         end }.
+Module Type ArcThreadSig.
+  Declare Module Arc : ArcSig.
+  Export Arc.
+  Module Base := Base Arc.
+  Export Base.
 
-      Fixpoint read_reg_slcs
-               (r : reg)
-               (rslcs : list reg_slc)
-               (pref : list decoded_instruction_state)
-               (rf : list (instruction_id * nat * reg_slc_val))
-        : option (list (instruction_id * nat * reg_slc_val)) :=
-        match pref with
-        | ins::pref =>
-          let wslcs := List.combine (List.seq 0 (List.length ins.(ins_reg_writes)))
-                                    ins.(ins_reg_writes) in
-          let wslcs := List.filter (fun '(i, w) => isTrue (w.(rws_slc_val).(rsv_slc).(rs_reg) = r))
-                                   wslcs in
-          let wslcs := List.map (fun '(i, w) => ((ins.(ins_id), i), w.(rws_slc_val))) wslcs in
+  Parameter  mem_read_request_cand : list decoded_instruction_state ->
+                                     decoded_instruction_state -> bool.
+End ArcThreadSig.
 
-          match Utils.reads_from_slcs wslcs rslcs rf with
-          | Some (rf, nil) => Some rf
-          | Some (rf, rslcs) => read_reg_slcs r rslcs pref rf
-          | None => None
-          end
-        | nil =>
-          (* FIXME: read initial value; for now read 0 *)
-          Some (List.fold_left (fun rf rslc =>
-                                  (InstructionID 0, 0, {| rsv_slc := rslc;
-                                            rsv_val :=
-                                              Some (wzero rslc.(rs_size)) |})::rf)
-                               rslcs
-                               rf)
-        end.
+Require SimpleA64InsSem.
 
-      Program Definition reg_val_of_reads_from (slc : reg_slc)
-                 (rf : list ((instruction_id * nat) * reg_slc_val))
-        : reg_val slc.(rs_size) :=
-        List.fold_left
-          (fun w '(_, rsv) =>
-             match rsv.(rsv_val) with
-             | Some val =>
-               if decide (rsv.(rsv_slc).(rs_size)
-                          <= slc.(rs_size) /\
-                          slc.(rs_first_bit)
-                          <= rsv.(rsv_slc).(rs_first_bit)) then
-                 let w' := zext val (slc.(rs_size) -
-                                     rsv.(rsv_slc).(rs_size)) in
-                 let w' := (w' ^<< (rsv.(rsv_slc).(rs_first_bit) -
-                                    slc.(rs_first_bit)))%word in
-                 wor w w'
-               else
-                 (* FIXME: this shouldn't be reachable *)
-                 w
-             | None =>
+Module SimpleArmv8A : ArcThreadSig with Module Arc := SimpleA64InsSem.Armv8A.
+  Module Arc := SimpleA64InsSem.Armv8A.
+  Export SimpleA64InsSem.Armv8A.
+  Module Base := Base SimpleA64InsSem.Armv8A.
+  Export Base.
+
+  Section InstructionKind.
+    Variable a : ast.
+
+    Definition is_strong_memory_barrier : bool := (* FIXME: *) let a := a in false.
+    Definition is_ld_barrier : bool := (* FIXME: *) let a := a in false.
+    Definition is_instruction_barrier : bool := (* FIXME: *) let a := a in false.
+
+    Definition is_load : bool :=
+      match a with
+      | Load _ _ _ => true
+      | _ => false
+      end.
+    Definition is_store_release : bool := (* FIXME: *) let a := a in false.
+    Definition is_load_acquire  : bool := (* FIXME: *) let a := a in false.
+  End InstructionKind.
+
+  Section PossibleReadsWrites.
+    Variable ins : decoded_instruction_state.
+
+    Definition read_initiated : bool := isTrue (ins.(ins_mem_reads) <> None).
+
+    Definition read_completed : bool :=
+      match ins.(ins_mem_reads) with
+      | Some reads => forallb (fun u => isTrue (u = nil))
+                             reads.(rs_unsat_slcs)
+      | None => false
+      end.
+
+    (* Definition read_requested rr : bool := *)
+    (*   List.lookup rr inst.subreads.sr_requested <> Nothing. *)
+
+
+    (* (* Return Nothing if the read footprint is not determined yet, or Just *)
+     (*    applied to the set of read addresses otherwise. If the memory read *)
+     (*    has already been initiated then this information is in the *)
+     (*    instruction instance state; if not, the footprint is only *)
+     (*    determined if the instruction has a Mem_read outcome in the next *)
+     (*    state. (This depends on the fact that the only register in the Sail *)
+     (*    code for loads is for determining the data, after that the read can *)
+     (*    go ahead. *) *)
+    (* let read_footprint_of_load instruction : maybe footprint = *)
+    (*   match instruction.subreads.sr_addr with *)
+    (*   | Just fp -> Just fp *)
+    (*   | Nothing -> *)
+    (*       match instruction.micro_op_state with *)
+    (*       | MOS_plain (O_Read_mem (read_kind,addr_lifted,size) _) -> *)
+    (*          let addr = ensure_just (address_of_address_lifted addr_lifted) *)
+    (*                       "read_footprint_of_load: bad address" in *)
+    (*          Just (addr, size) *)
+    (*       | _ ->  Nothing *)
+    (*       end *)
+    (*   end *)
+
+
+    (* let possibly_reads_address *)
+    (*     (instruction: instruction_instance 'i) *)
+    (*     (fps:         set footprint) *)
+    (*     : bool *)
+    (*   = *)
+    (*   is_memory_load_instruction (ik instruction) && *)
+    (*   match read_footprint_of_load instruction with *)
+    (*   | Just fp -> non_empty_intersection_set fps {fp} *)
+    (*   | Nothing -> exists ((_, s) IN fps). s <> 0 *)
+    (*   end *)
+
+
+    (* let possibly_writes_address *)
+    (*     (instruction: instruction_instance 'i) *)
+    (*     (fps:         set footprint) *)
+    (*     : bool *)
+    (*   = *)
+    (*   is_viable_memory_store_ii instruction && *)
+    (*   match instruction.subwrites.sw_addr with *)
+    (*   | Just fp -> non_empty_intersection_set fps {fp} *)
+    (*   | Nothing -> exists ((_, s) IN fps). s <> 0 *)
+    (*   end *)
+
+
+    (* (* Return 'true' iff 'instruction' might read or write from/to a footprint *)
+     (* intersecting with 'fps'. In particular, return 'true' if the footprint of *)
+     (* 'instruction' can't be determined. *)
+     (* NOTE: we check the instruction in its current state, i.e., if the *)
+     (* pseudocode has not made enough steps yet to make the reads/writes avilable *)
+     (* the function returns 'true' for any (non-empty) 'fps', and we don't consider *)
+     (* what can happen if the instruction is restarted. *) *)
+    (* let possibly_reads_or_writes_address *)
+    (*     (inst: instruction_instance 'i) *)
+    (*     (fps:  set footprint) *)
+    (*     : bool *)
+    (*   = *)
+    (*   possibly_reads_address inst fps || possibly_writes_address inst fps *)
+
+    (* return true iff the sail code has already generated its memory-read event for *)
+    (*    the instruction. This guarantees that the instruction's memory read is *)
+    (*    recorded in the instruction_instance state. *)
+    Definition all_reads_are_calculated : bool :=
+      is_load ins.(ins_ast)
+                    ---> read_initiated.
+
+    (* let all_writes_are_calculated inst : bool = *)
+    (*   is_viable_memory_store_ii inst --> write_initiated inst *)
+
+    (* (* return true iff the sail code has already generated all the memory-read/write *)
+     (*    events (except AArch64 write-mem-value, i.e., E_write_memv) for the *)
+     (*    instruction. This guarantees that any memory read/write footprint of the *)
+     (*    instruction is recorded in the instruction_instance state. *) *)
+    (* let all_writes_reads_are_calculated inst : bool = *)
+    (*   (* for efficiency, first check if 'inst' is unfinished *) *)
+    (*   inst.finished || *)
+    (*   (all_reads_are_calculated inst && all_writes_are_calculated inst) *)
+
+    Definition is_entirely_satisfied_load : bool :=
+      all_reads_are_calculated
+      && read_completed.
+
+    Definition finished_load_part : bool :=
+      ins.(ins_finished). (* || ins.rmw_finished_load_snapshot <> Nothing *)
+  End PossibleReadsWrites.
+
+
+
+
+  Open Scope bool_scope.
+  (* LEM: machineDefThreadSubsystem.lem: pop_memory_read_request_cand *)
+  Definition mem_read_request_cand (pref : list decoded_instruction_state)
+             (ins : decoded_instruction_state) : bool :=
+    (* NOTE: we don't check that po-preceding instructions to the same
+                 address are finished.
+                 See also private comment THREAD1 *)
+    (forallb (fun prev_ins =>
+               is_strong_memory_barrier prev_ins.(ins_ast)
+               ---> prev_ins.(ins_finished))
+            pref) &&
+
+    (* See private comment THREAD2 *)
+    (forallb (fun prev_ins =>
+               is_instruction_barrier prev_ins.(ins_ast)
+               ---> prev_ins.(ins_finished))
+            pref) &&
+
+    (* barrier.st/ld: *)
+    (forallb (fun prev_ins =>
+               is_ld_barrier prev_ins.(ins_ast)
+               ---> prev_ins.(ins_finished))
+            pref) &&
+
+    (* load-acquire/store-release (RCsc):
+           A store-release and a po-succeeding load-acquire are observed in
+           program order *)
+    (is_load_acquire ins.(ins_ast)
+     ---> forallb (fun prev_ins =>
+                 is_store_release prev_ins.(ins_ast)
+                 ---> prev_ins.(ins_finished))
+              pref) &&
+
+    (* All po-preceding load-acquires must issue their requests before the
+         read request.
+         Also see private note THREAD3 *)
+    (forallb (fun prev_ins =>
+               is_load_acquire prev_ins.(ins_ast)
+               ---> (finished_load_part prev_ins ||
+                  is_entirely_satisfied_load prev_ins))
+            pref).
+
+End SimpleArmv8A.
+
+(******************************************************************************)
+
+Module Make (Arc : ArcSig) (ArcThread : ArcThreadSig with Module Arc := Arc) : ThreadSig Arc.
+  Export ArcThread.
+
+  Definition state := state.
+  Definition showable_state := showable_state.
+  Definition E := E.
+  Definition showable_E := showable_E.
+  Definition is_eager_event {A T} := @is_eager_event A T.
+  Definition denote {F} := @denote F.
+
+  Definition initial_state '((InstructionID iid) : instruction_id) (loc : mem_loc)
+    : state :=
+    {| next_iid := InstructionID (iid + 1);
+       instruction_tree := TLeaf (TNode (InstructionID iid, loc) []) |}.
+
+  Section RegisterRead.
+    Local Instance slice_id_rsv : Slice (instruction_id * nat * reg_slc_val) :=
+      { start := fun '(_, _, s) => Utils.start s;
+        size := fun '(_, _, s) => Utils.size s;
+        sub_slice := fun '(id, s) start size =>
+                       match sub_slice s start size with
+                       | Some s' => Some (id, s')
+                       | None => None
+                       end }.
+
+    Fixpoint read_reg_slcs
+             (r : reg)
+             (rslcs : list reg_slc)
+             (pref : list decoded_instruction_state)
+             (rf : list (instruction_id * nat * reg_slc_val))
+      : option (list (instruction_id * nat * reg_slc_val)) :=
+      match pref with
+      | ins::pref =>
+        let wslcs := List.combine (List.seq 0 (List.length ins.(ins_reg_writes)))
+                                  ins.(ins_reg_writes) in
+        let wslcs := List.filter (fun '(i, w) => isTrue (w.(rws_slc_val).(rsv_slc).(rs_reg) = r))
+                                 wslcs in
+        let wslcs := List.map (fun '(i, w) => ((ins.(ins_id), i), w.(rws_slc_val))) wslcs in
+
+        match Utils.reads_from_slcs wslcs rslcs rf with
+        | Some (rf, nil) => Some rf
+        | Some (rf, rslcs) => read_reg_slcs r rslcs pref rf
+        | None => None
+        end
+      | nil =>
+        (* FIXME: read initial value; for now read 0 *)
+        Some (List.fold_left (fun rf rslc =>
+                                (InstructionID 0, 0, {| rsv_slc := rslc;
+                                                        rsv_val :=
+                                                          Some (wzero rslc.(rs_size)) |})::rf)
+                             rslcs
+                             rf)
+      end.
+
+    Program Definition reg_val_of_reads_from (slc : reg_slc)
+            (rf : list ((instruction_id * nat) * reg_slc_val))
+      : reg_val slc.(rs_size) :=
+      List.fold_left
+        (fun w '(_, rsv) =>
+           match rsv.(rsv_val) with
+           | Some val =>
+             if decide (rsv.(rsv_slc).(rs_size)
+                        <= slc.(rs_size) /\
+                        slc.(rs_first_bit)
+                        <= rsv.(rsv_slc).(rs_first_bit)) then
+               let w' := zext val (slc.(rs_size) -
+                                   rsv.(rsv_slc).(rs_size)) in
+               let w' := (w' ^<< (rsv.(rsv_slc).(rs_first_bit) -
+                                  slc.(rs_first_bit)))%word in
+               wor w w'
+             else
                (* FIXME: this shouldn't be reachable *)
                w
-             end)
-          rf (wzero slc.(rs_size)).
-      Obligation 1.
-      rewrite Nat.add_comm. apply Nat.sub_add. auto.
-      Qed.
-    End RegisterRead.
+           | None =>
+             (* FIXME: this shouldn't be reachable *)
+             w
+           end)
+        rf (wzero slc.(rs_size)).
+    Obligation 1.
+    rewrite Nat.add_comm. apply Nat.sub_add. auto.
+    Qed.
+  End RegisterRead.
 
-    Fixpoint get_first_unfetched_instruction_helper
-             (iid : instruction_id)
-             (pref : list decoded_instruction_state)
-             (t : ins_tree)
-      : option (list decoded_instruction_state * mem_loc *
-                list (tree (instruction_id * mem_loc) unit)) :=
-      match t with
-      | TNode i ts =>
+  Fixpoint get_first_unfetched_instruction_helper
+           (iid : instruction_id)
+           (pref : list decoded_instruction_state)
+           (t : ins_tree)
+    : option (list decoded_instruction_state * mem_loc *
+              list (tree (instruction_id * mem_loc) unit)) :=
+    match t with
+    | TNode i ts =>
+      match List.find (fun x => isTrue (~(x = None)))
+                      (List.map (get_first_unfetched_instruction_helper iid (i::pref)) ts)
+      with
+      | Some x => x
+      | None => None
+      end
+    | TLeaf (TNode (iid', loc) ts) =>
+      if decide (iid' = iid) then Some (pref, loc, ts)
+      else None
+    | TLeaf _ => None
+    end.
+
+  Definition get_first_unfetched_instruction
+             (iid : instruction_id) (s : state)
+    : option (list decoded_instruction_state * mem_loc *
+              list (tree (instruction_id * mem_loc) unit)) :=
+    get_first_unfetched_instruction_helper iid [] s.(instruction_tree).
+
+  Fixpoint get_dec_instruction_state_helper
+           (iid : instruction_id)
+           (pref : list decoded_instruction_state)
+           (t : ins_tree)
+    : option (list decoded_instruction_state *
+              decoded_instruction_state *
+              list ins_tree) :=
+    match t with
+    | TNode i ts =>
+      if decide (i.(ins_id) = iid) then Some (pref, i, ts)
+      else
         match List.find (fun x => isTrue (~(x = None)))
-                        (List.map (get_first_unfetched_instruction_helper iid (i::pref)) ts)
+                        (List.map (get_dec_instruction_state_helper iid (i::pref)) ts)
         with
         | Some x => x
         | None => None
         end
-      | TLeaf (TNode (iid', loc) ts) =>
-        if decide (iid' = iid) then Some (pref, loc, ts)
-        else None
-      | TLeaf _ => None
-      end.
+    | TLeaf _ => None
+    end.
 
-    Definition get_first_unfetched_instruction
-               (iid : instruction_id) (s : state)
-      : option (list decoded_instruction_state * mem_loc *
-                list (tree (instruction_id * mem_loc) unit)) :=
-      get_first_unfetched_instruction_helper iid [] s.(instruction_tree).
+  Definition get_dec_instruction_state
+             (iid : instruction_id) (s : state)
+    : option (list decoded_instruction_state *
+              decoded_instruction_state *
+              list ins_tree) :=
+    get_dec_instruction_state_helper iid [] s.(instruction_tree).
 
-    Fixpoint get_dec_instruction_state_helper
-               (iid : instruction_id)
-               (pref : list decoded_instruction_state)
-               (t : ins_tree)
-      : option (list decoded_instruction_state *
-                decoded_instruction_state *
-                list ins_tree) :=
-      match t with
-      | TNode i ts =>
-        if decide (i.(ins_id) = iid) then Some (pref, i, ts)
-        else
-          match List.find (fun x => isTrue (~(x = None)))
-                          (List.map (get_dec_instruction_state_helper iid (i::pref)) ts)
-          with
-          | Some x => x
-          | None => None
-          end
-      | TLeaf _ => None
-      end.
+  Definition try_get_dec_instruction_state {F}
+             `{exceptE error -< F}
+             (iid : instruction_id) (s : state)
+    : itree F (list decoded_instruction_state *
+               decoded_instruction_state *
+               list ins_tree) :=
+    try_unwrap_option (get_dec_instruction_state iid s)
+                      ("try_get_dec_instruction_state: missing iid " ++ show iid).
 
-    Definition get_dec_instruction_state
-               (iid : instruction_id) (s : state)
-      : option (list decoded_instruction_state *
-                decoded_instruction_state *
-                list ins_tree) :=
-      get_dec_instruction_state_helper iid [] s.(instruction_tree).
+  Definition update_dec_instruction_state_and_subts
+             (iid : instruction_id) (dins : decoded_instruction_state)
+             (ts : list ins_tree) (s : state)
+    : state :=
+    let fix helper t :=
+        match t with
+        | TNode i ts' =>
+          if decide (i.(ins_id) = iid) then TNode dins ts
+          else TNode i (List.map helper ts')
+        | TLeaf (TNode (iid', _) _) =>
+          if decide (iid' = iid) then TNode dins ts
+          else t
+        | TLeaf (TLeaf tt) => t
+        end in
+    s <| instruction_tree := helper s.(instruction_tree) |>.
 
-    Definition try_get_dec_instruction_state {F}
-               `{exceptE error -< F}
-               (iid : instruction_id) (s : state)
-      : itree F (list decoded_instruction_state *
-                 decoded_instruction_state *
-                 list ins_tree) :=
-      try_unwrap_option (get_dec_instruction_state iid s)
-                        ("try_get_dec_instruction_state: missing iid " ++ show iid).
+  Definition update_dec_instruction_state
+             (iid : instruction_id) (dins : decoded_instruction_state)
+             (s : state)
+    : state :=
+    let fix helper t :=
+        match t with
+        | TNode i ts' =>
+          if decide (i.(ins_id) = iid) then TNode dins ts'
+          else TNode i (List.map helper ts')
+        | TLeaf (TNode (iid', _) ts') =>
+          if decide (iid' = iid) then TNode dins (List.map TLeaf ts')
+          else t
+        | TLeaf (TLeaf tt) => t
+        end in
+    s <| instruction_tree := helper s.(instruction_tree) |>.
 
-    Definition update_dec_instruction_state_and_subts
-               (iid : instruction_id) (dins : decoded_instruction_state)
-               (ts : list ins_tree) (s : state)
-      : state :=
-      let fix helper t :=
-          match t with
-          | TNode i ts' =>
-            if decide (i.(ins_id) = iid) then TNode dins ts
-            else TNode i (List.map helper ts')
-          | TLeaf (TNode (iid', _) _) =>
-            if decide (iid' = iid) then TNode dins ts
-            else t
-          | TLeaf (TLeaf tt) => t
-          end in
-      s <| instruction_tree := helper s.(instruction_tree) |>.
+  Section Handle_instruction_instance.
+    Context {F : Type -> Type}.
+    Context `{storageE -< F}.
+    Context `{stateE state -< F}.
+    Context `{exceptE disabled -< F}.
+    Context `{exceptE error -< F}.
+    Context `{debugE -< F}.
 
-    Definition update_dec_instruction_state
-               (iid : instruction_id) (dins : decoded_instruction_state)
-               (s : state)
-      : state :=
-      let fix helper t :=
-          match t with
-          | TNode i ts' =>
-            if decide (i.(ins_id) = iid) then TNode dins ts'
-            else TNode i (List.map helper ts')
-          | TLeaf (TNode (iid', _) ts') =>
-            if decide (iid' = iid) then TNode dins (List.map TLeaf ts')
-            else t
-          | TLeaf (TLeaf tt) => t
-          end in
-      s <| instruction_tree := helper s.(instruction_tree) |>.
+    Variable iid : instruction_id.
 
-    Section Handle_instruction_instance.
-      Context {F : Type -> Type}.
-      Context `{storageE -< F}.
-      Context `{stateE state -< F}.
-      Context `{exceptE disabled -< F}.
-      Context `{exceptE error -< F}.
-      Context `{debugE -< F}.
+    Definition try_fetch_and_decode_or_restart
+      : itree F (list instruction_id * ast) :=
+      s <- get
+      ;; match get_dec_instruction_state iid s with
+         | Some (_, ins, _) =>
+           (* Nothing to do, the instruction-state has already been restarted. *)
+           ret ([], ins.(ins_ast))
+         | None =>
+           '(_, loc, _) <- guard_some (get_first_unfetched_instruction iid s)
+           ;; '(slc, rf) <- trigger (StEReadInstruction loc)
+           ;; val <- try_unwrap_option (mem_slc_val_of_reads_from slc rf)
+                                      "try_fetch_and_decode_or_restart: some bytes are missing from memory read of instruction."
+           ;; ast <- try_unwrap_option (decode val)
+                                      "try_fetch_and_decode_or_restart: decoding of instruction failed"
+           ;; let ins := initial_decoded_instruction_state iid loc ast in
+              let next_pcs := next_pc loc ast in
+              let '(InstructionID niid) := s.(next_iid) in
+              let iids :=
+                  List.map InstructionID
+                           (List.seq niid (List.length next_pcs)) in
+              let subts := List.map (fun '(iid, pc) => TLeaf (TNode (iid, pc) []))
+                                    (List.combine iids next_pcs) in
+              let s := s <| next_iid := InstructionID (niid + (List.length next_pcs)) |> in
+              let s := update_dec_instruction_state_and_subts iid ins subts s in
+              'tt <- put s
+              ;; ret (iids, ast)
+         end.
 
-      Variable iid : instruction_id.
+    Definition try_finish_instruction : itree F unit :=
+      (* FIXME: check finish condition *)
+      s <- get
+      ;; '(pref, ins, _) <- try_get_dec_instruction_state iid s
+      ;; let ins := ins <| ins_finished := true |> in
+         let s := update_dec_instruction_state iid ins s in
+         put s.
 
-      Definition try_fetch_and_decode_or_restart
-        : itree F (list instruction_id * ast) :=
-        s <- get
-        ;; match get_dec_instruction_state iid s with
-           | Some (_, ins, _) =>
-             (* Nothing to do, the instruction-state has already been restarted. *)
-             ret ([], ins.(ins_ast))
-           | None =>
-             '(_, loc, _) <- guard_some (get_first_unfetched_instruction iid s)
-             ;; '(slc, rf) <- trigger (StEReadInstruction loc)
-             ;; val <- try_unwrap_option (mem_slc_val_of_reads_from slc rf)
-                                        "try_fetch_and_decode_or_restart: some bytes are missing from memory read of instruction."
-             ;; ast <- try_unwrap_option (decode val)
-                                        "try_fetch_and_decode_or_restart: decoding of instruction failed"
-             ;; let ins := initial_decoded_instruction_state iid loc ast in
-                let next_pcs := next_pc loc ast in
-                let '(InstructionID niid) := s.(next_iid) in
-                let iids :=
-                    List.map InstructionID
-                             (List.seq niid (List.length next_pcs)) in
-                let subts := List.map (fun '(iid, pc) => TLeaf (TNode (iid, pc) []))
-                                      (List.combine iids next_pcs) in
-                let s := s <| next_iid := InstructionID (niid + (List.length next_pcs)) |> in
-                let s := update_dec_instruction_state_and_subts iid ins subts s in
-                'tt <- put s
-             ;; ret (iids, ast)
-           end.
-
-      Definition try_finish_instruction : itree F unit :=
-        (* FIXME: check finish condition *)
-        s <- get
-        ;; '(pref, ins, _) <- try_get_dec_instruction_state iid s
-        ;; let ins := ins <| ins_finished := true |> in
-           let s := update_dec_instruction_state iid ins s in
-           put s.
-
-      Definition try_read_reg_slc (rslc : reg_slc)
-        : itree F (reg_val rslc.(rs_size)) :=
-        s <- get
-        ;; '(pref, ins, _) <- try_get_dec_instruction_state iid s
-        ;; match read_reg_slcs rslc.(rs_reg) [rslc] pref [] with
-           | Some rf =>
-             let val := reg_val_of_reads_from rslc rf in
-             let reg_reads :=
-                 List.map
-                   (fun rrs =>
-                      if decide (rrs.(rrs_slc) = rslc) then
-                        mk_reg_read_state rslc rrs.(rrs_feeding_addr) rf (Some val)
-                      else rrs)
-                   ins.(ins_reg_reads) in
-             let ins := ins <| ins_reg_reads := reg_reads |> in
-             let s := update_dec_instruction_state iid ins s in
-             'tt <- put s
-             ;; ret val
-           | None => throw (Disabled tt)
-           end.
-
-      Definition try_write_reg_slc (rslc : reg_slc)
-                 (val : reg_val rslc.(rs_size))
-        : itree F unit :=
-        s <- get
-        ;; '(_, ins, _) <- try_get_dec_instruction_state iid s
-        ;; let reg_writes :=
+    Definition try_read_reg_slc (rslc : reg_slc)
+      : itree F (reg_val rslc.(rs_size)) :=
+      s <- get
+      ;; '(pref, ins, _) <- try_get_dec_instruction_state iid s
+      ;; match read_reg_slcs rslc.(rs_reg) [rslc] pref [] with
+         | Some rf =>
+           let val := reg_val_of_reads_from rslc rf in
+           let reg_reads :=
                List.map
-                 (fun rws =>
-                    if decide (rws.(rws_slc_val).(rsv_slc) = rslc) then
-                      let rdf := List.concat (List.map (fun rrs => List.map fst rrs.(rrs_reads_from))
-                                                       ins.(ins_reg_reads)) in
-                      let mdf := match ins.(ins_mem_reads) with Some _ => true | _ => false end in
-                      mk_reg_write_state {| rsv_slc := rslc; rsv_val := Some val |}
-                                         rdf mdf
-                    else rws)
-                 ins.(ins_reg_writes) in
-           let ins := ins <| ins_reg_writes := reg_writes |> in
+                 (fun rrs =>
+                    if decide (rrs.(rrs_slc) = rslc) then
+                      mk_reg_read_state rslc rrs.(rrs_feeding_addr) rf (Some val)
+                    else rrs)
+                 ins.(ins_reg_reads) in
+           let ins := ins <| ins_reg_reads := reg_reads |> in
            let s := update_dec_instruction_state iid ins s in
-           put s.
+           'tt <- put s
+           ;; ret val
+         | None => throw (Disabled tt)
+         end.
 
-      Definition handle_reg_access : regE ~> itree F :=
-        fun _ e =>
+    Definition try_write_reg_slc (rslc : reg_slc)
+               (val : reg_val rslc.(rs_size))
+      : itree F unit :=
+      s <- get
+      ;; '(_, ins, _) <- try_get_dec_instruction_state iid s
+      ;; let reg_writes :=
+             List.map
+               (fun rws =>
+                  if decide (rws.(rws_slc_val).(rsv_slc) = rslc) then
+                    let rdf := List.concat (List.map (fun rrs => List.map fst rrs.(rrs_reads_from))
+                                                     ins.(ins_reg_reads)) in
+                    let mdf := match ins.(ins_mem_reads) with Some _ => true | _ => false end in
+                    mk_reg_write_state {| rsv_slc := rslc; rsv_val := Some val |}
+                                       rdf mdf
+                  else rws)
+               ins.(ins_reg_writes) in
+         let ins := ins <| ins_reg_writes := reg_writes |> in
+         let s := update_dec_instruction_state iid ins s in
+         put s.
+
+    Definition handle_reg_access : regE ~> itree F :=
+      fun _ e =>
+        match e with
+        | RegERead rslc => try_read_reg_slc rslc
+        | RegEWrite rslc rval => try_write_reg_slc rslc rval
+        end.
+
+    Definition try_init_mem_load_ops (slc : mem_slc)
+      : itree F (list mem_read_id) :=
+      s <- get
+      ;; '(_, ins, _) <- try_get_dec_instruction_state iid s
+      ;; let sub_slcs := split_load_mem_slc ins.(ins_ast) slc in
+         let kind := mem_read_kind_of_ast ins.(ins_ast) in
+         let rids := List.map MemReadID
+                              (List.seq 0 (List.length sub_slcs)) in
+         let reads := List.map
+                        (fun '(rid, slc) => {| read_id := rid;
+                                            read_footprint := slc;
+                                            read_kind := kind |})
+                        (List.combine rids sub_slcs) in
+         let rs := {| rs_footprint := slc;
+                      rs_reads := reads;
+                      rs_unsat_slcs := List.map (fun r => [r.(read_footprint)]) reads;
+                      rs_reads_from := List.map (fun _ => nil) reads |} in
+         let ins := ins <| ins_mem_reads := Some rs |> in
+         let s := update_dec_instruction_state iid ins s in
+         'tt <- put s
+         ;; ret rids.
+
+
+    Definition try_sat_mem_load_op_forwarding (rid : mem_read_id)
+      : itree F (bool * list instruction_id) :=
+      (* FIXME: *)
+      let iid := iid in
+      guard false
+      ;; ret (false, []).
+
+    Definition restart_instructions (iids : list instruction_id)
+               (ts : list ins_tree)
+      : list ins_tree :=
+      List.map (tree_map
+                  (fun ins => if decide (In ins.(ins_id) iids) then
+                             (initial_decoded_instruction_state iid ins.(ins_loc) ins.(ins_ast))
+                           else ins)
+                  (fun l => l))
+               ts.
+
+    Definition try_sat_mem_load_op_from_storage '((MemReadID rid) : mem_read_id)
+      : itree F (list instruction_id) :=
+      s <- get
+      ;; '(pref, ins, subts) <- try_get_dec_instruction_state iid s
+      ;; 'tt <- guard (ArcThread.mem_read_request_cand pref ins)
+      ;; rs <- try_unwrap_option ins.(ins_mem_reads)
+                                      "try_sat_mem_load_op_from_storage: no mem reads."
+      ;; unsat_slcs <- try_unwrap_option (List.nth_error rs.(rs_unsat_slcs) rid)
+                                        "try_sat_mem_load_op_from_storage: missing rid."
+      (* ;; guard (isTrue (unsat_slcs <> [])) *)
+      ;; rr <- try_unwrap_option (List.nth_error rs.(rs_reads) rid)
+                                "try_sat_mem_load_op_from_storage: missing rid"
+      ;; rf_forward <- try_unwrap_option (List.nth_error rs.(rs_reads_from) rid)
+                                        "try_sat_mem_load_op_from_storage: missing rid."
+      ;; rf_storage <- trigger (StERead rr unsat_slcs)
+      ;; let rs := rs <| rs_unsat_slcs := list_replace_nth rid [] rs.(rs_unsat_slcs) |>
+                                                                                     <| rs_reads_from := list_replace_nth rid (rf_forward ++ rf_storage)
+                                                                                                                          rs.(rs_reads_from) |> in
+         let ins := ins <| ins_mem_reads := Some rs |> in
+         (* FIXME: compute iids that need to be restarted *)
+         let restarts :=
+             (List.fold_left (fun iids t =>
+                                List.fold_left (fun iids i =>
+                                                  match i with
+                                                  | inl ins =>
+                                                    if ins.(ins_finished) then iids
+                                                    else ins.(ins_id) :: iids
+                                                  | inr _ => iids
+                                                  end)
+                                               (tree_to_list_preorder t)
+                                               iids)
+                             subts
+                             []) in
+         let subts := restart_instructions restarts subts in
+         let s := update_dec_instruction_state_and_subts iid ins subts s in
+         'tt <- put s
+         ;; ret restarts.
+
+    Definition try_complete_load_ops : itree F mem_slc_val :=
+      s <- get
+      ;; '(_, ins, _) <- try_get_dec_instruction_state iid s
+      ;; rs <- try_unwrap_option ins.(ins_mem_reads)
+                                      "try_complete_load_ops: no mem reads."
+      (* ;; guard (isTrue (Forall (fun u => u = []) rs.(rs_unsat_slcs))) *)
+      ;; val <- try_unwrap_option
+                 (mem_slc_val_of_reads_from
+                    rs.(rs_footprint)
+                         (List.concat rs.(rs_reads_from)))
+                 "try_complete_load_ops: some bytes are missing from memory read."
+      ;; ret val.
+
+    Definition try_init_mem_store_op_fps (slc : mem_slc) : itree F unit :=
+      s <- get
+      ;; '(_, ins, _) <- try_get_dec_instruction_state iid s
+      ;; let ws := {| ws_footprint := slc;
+                      ws_writes := [];
+                      ws_has_propagated := [] |} in
+         let ins := ins <| ins_mem_writes := Some ws |> in
+         let s := update_dec_instruction_state iid ins s in
+         put s.
+
+    Definition try_insta_mem_store_op_vals (val : mem_slc_val) : itree F unit :=
+      s <- get
+      ;; '(_, ins, _) <- try_get_dec_instruction_state iid s
+      ;; ws <- try_unwrap_option ins.(ins_mem_writes)
+                                      "try_insta_mem_store_op_vals: no mem writes"
+      ;; let sub_slcs := split_store_mem_slc_val ins.(ins_ast) ws.(ws_footprint) val in
+         let kind := mem_write_kind_of_ast ins.(ins_ast) in
+         let wids := List.seq 0 (List.length sub_slcs) in
+         let writes := List.map
+                         (fun '(wid, (slc, val)) => {| write_id := MemWriteID wid;
+                                                    write_footprint := slc;
+                                                    write_val := val;
+                                                    write_kind := kind |})
+                         (List.combine wids sub_slcs) in
+         let ws := ws <| ws_writes := writes |>
+                                             <| ws_has_propagated := List.map (fun _ => false) writes |>in
+         let ins := ins <| ins_mem_writes := Some ws |> in
+         let s := update_dec_instruction_state iid ins s in
+         put s.
+
+    Definition try_commit_store_instruction : itree F (list mem_write_id) :=
+      s <- get
+      ;; '(_, ins, _) <- try_get_dec_instruction_state iid s
+      ;; ws <- try_unwrap_option ins.(ins_mem_writes)
+                                      "try_commit_store_instruction: no mem writes"
+      (* FIXME: check commit-store condition *)
+      ;; let wids := List.map write_id ws.(ws_writes) in
+         ret wids.
+
+    Definition try_propagate_store_op '((MemWriteID wid) : mem_write_id)
+      : itree F (list instruction_id) :=
+      s <- get
+      ;; '(_, ins, subts) <- try_get_dec_instruction_state iid s
+      ;; ws <- try_unwrap_option ins.(ins_mem_writes)
+                                      "try_propagate_store_op: no mem writes"
+      (* ;; guard (isTrue (List.nth_error ws.(ws_has_propagated) wid = Some false)) *)
+      ;; w <- try_unwrap_option (List.nth_error ws.(ws_writes) wid)
+                               "try_propagate_store_op: missing wid"
+      (* FIXME: check mem-write-propagation condition *)
+      ;; 'tt <- trigger (StEWrite w)
+      ;; let ws := ws <| ws_has_propagated := list_replace_nth wid true ws.(ws_has_propagated) |> in
+         let ins := ins <| ins_mem_writes := Some ws |> in
+         (* FIXME: compute iids that need to be restarted *)
+         let restarts :=
+             (List.fold_left (fun iids t =>
+                                List.fold_left (fun iids i =>
+                                                  match i with
+                                                  | inl ins =>
+                                                    if ins.(ins_finished) then iids
+                                                    else ins.(ins_id) :: iids
+                                                  | inr _ => iids
+                                                  end)
+                                               (tree_to_list_preorder t)
+                                               iids)
+                             subts
+                             []) in
+         let subts := restart_instructions restarts subts in
+         let s := update_dec_instruction_state_and_subts iid ins subts s in
+         'tt <- put s
+         ;; ret restarts.
+
+    Definition try_complete_store_ops : itree F unit :=
+      (* FIXME: is there anything we need to check here? *)
+      let iid := iid in
+      ret tt.
+
+  End Handle_instruction_instance.
+
+  Definition handle_E {F}
+             `{storageE -< F}
+             `{stateE state -< F}
+             `{exceptE disabled -< F}
+             `{exceptE error -< F}
+             `{debugE -< F}
+             (iid : instruction_id)
+    : E ~> itree F :=
+    fun A e =>
+      let it : itree F A :=
           match e with
-          | RegERead rslc => try_read_reg_slc rslc
-          | RegEWrite rslc rval => try_write_reg_slc rslc rval
-          end.
-
-      Definition try_init_mem_load_ops (slc : mem_slc)
-        : itree F (list mem_read_id) :=
-        s <- get
-        ;; '(_, ins, _) <- try_get_dec_instruction_state iid s
-        ;; let sub_slcs := split_load_mem_slc ins.(ins_ast) slc in
-           let kind := mem_read_kind_of_ast ins.(ins_ast) in
-           let rids := List.map MemReadID
-                                (List.seq 0 (List.length sub_slcs)) in
-           let reads := List.map
-                          (fun '(rid, slc) => {| read_id := rid;
-                                              read_footprint := slc;
-                                              read_kind := kind |})
-                          (List.combine rids sub_slcs) in
-           let rs := {| rs_footprint := slc;
-                        rs_reads := reads;
-                        rs_unsat_slcs := List.map (fun r => [r.(read_footprint)]) reads;
-                        rs_reads_from := List.map (fun _ => nil) reads |} in
-           let ins := ins <| ins_mem_reads := Some rs |> in
-           let s := update_dec_instruction_state iid ins s in
-           'tt <- put s
-           ;; ret rids.
-
-
-      Definition try_sat_mem_load_op_forwarding (rid : mem_read_id)
-        : itree F (bool * list instruction_id) :=
-        (* FIXME: *)
-        let iid := iid in
-        guard false
-        ;; ret (false, []).
-
-      Definition restart_instructions (iids : list instruction_id)
-                 (ts : list ins_tree)
-        : list ins_tree :=
-        List.map (tree_map
-                    (fun ins => if decide (In ins.(ins_id) iids) then
-                               (initial_decoded_instruction_state iid ins.(ins_loc) ins.(ins_ast))
-                             else ins)
-                    (fun l => l))
-                 ts.
-
-      (* Notation "'forall' ( x 'MEM' l ), p" := (Forall (fun x => p) l) *)
-      (*                                           (at level 40) : . *)
-      (* Notation "'forall' ( ' x  'MEM' l ), p" := (Forall (fun x => p) l) *)
-      (*                                         (x pattern, at level 40). *)
-
-      Infix "-->" := implb (at level 51, right associativity)
-                     : bool_scope.
-      (* LEM: machineDefThreadSubsystem.lem: pop_memory_read_request_cand *)
-  (*     Definition mem_read_request_cand pref i : Prop := *)
-  (*       (* NOTE: we don't check po-previous instructions to the same address. *)
-  (*          See also private comment THREAD1 *) *)
-  (*       (forallb (fun `(_, _, prev_ins) => *)
-  (*                     is_strong_memory_barrier prev_ins.(ins_ast) *)
-  (*                     --> prev_inst.(ins_finished)) *)
-  (*               pref) *)
-
-  (*       (forall (prev_inst MEM pref), *)
-  (*          is_pop_strong_memory_barrier prev_inst.(ins_ast) --> prev_inst.(ins_finished)) && *)
-
-  (* (* See private comment THREAD2 *) *)
-  (* (forall (prev_inst MEM inst_context.active_prefix). *)
-  (*      is_pop_instruction_barrier (ik prev_inst) --> prev_inst.finished) && *)
-
-  (* (* Additions for barrier.st/ld: *) *)
-  (* (forall (prev_inst MEM inst_context.active_prefix). *)
-  (*     is_AArch64_ld_barrier (ik prev_inst) --> prev_inst.finished) && *)
-
-  (* (* Additions for load.acquire/store.release: *) *)
-  (* (* A Store-Release followed by a Load-Acquire is observed in program order *) *)
-  (* ((is_AArch64_load_acquire (ik instruction) || *)
-  (*   is_RISCV_load_strong_acquire (ik instruction)) --> *)
-  (*     forall (prev_inst MEM inst_context.active_prefix). *)
-  (*         (is_AArch64_store_release (ik prev_inst) || *)
-  (*          is_RISCV_store_strong_release (ik prev_inst)) *)
-  (*         --> prev_inst.finished) && *)
-
-  (* (* All po-previous Load-acquires must issue their requests before the *)
-  (* read request. Also see private note THREAD3 *) *)
-  (* (forall (prev_inst MEM inst_context.active_prefix). *)
-  (*     (is_AArch64_load_acquire (ik prev_inst) || *)
-  (*        is_RISCV_load_acquire (ik prev_inst)) *)
-  (*     --> *)
-  (*     (finished_load_part prev_inst || *)
-  (*     is_entirely_satisfied_load prev_inst)) && *)
-
-  (* (* Additions for lwsync: *) *)
-  (* (* all loads that are po-followed by lwsync in active_prefix are finished *) *)
-  (* List.dropWhile (fun i -> not (is_lwsync (ik i))) inst_context.active_prefix *)
-  (* $> List.dropWhile (fun i -> is_memory_load_instruction (ik i) --> finished_load_part i) *)
-  (* $> List.null && *)
-
-  (* (* Additions for load-reserve/store-conditional: *) *)
-  (* (is_PPC_load_reserve (ik instruction) --> *)
-  (*     forall (prev_inst MEM inst_context.active_prefix). *)
-  (*         (is_PPC_load_reserve (ik prev_inst) || is_PPC_store_conditional (ik prev_inst)) *)
-  (*         --> prev_inst.finished) && *)
-
-  (* (*** Additions for RISCV fences ***) *)
-  (* (forall_iprev_with_prefix inst_context.active_prefix $ fun prev_inst prev_active_prefix -> *)
-  (*     is_RISCV_fence_sr (ik prev_inst) --> *)
-  (*       (prev_inst.finished || *)
-  (*       (is_RISCV_fence_pr (ik prev_inst) *)
-  (*         && not (is_RISCV_fence_pw (ik prev_inst)) *)
-  (*         && forall (prev_prev_inst MEM prev_active_prefix). *)
-  (*               is_memory_load_instruction (ik prev_prev_inst) *)
-  (*                 --> is_entirely_satisfied_load prev_prev_inst))) && *)
-
-  (* (forall_iprev_with_prefix inst_context.active_prefix $ fun prev_inst prev_active_prefix -> *)
-  (*     is_RISCV_fence_tso (ik prev_inst) --> *)
-  (*       (prev_inst.finished || *)
-  (*       forall (prev_prev_inst MEM prev_active_prefix). *)
-  (*           is_memory_load_instruction (ik prev_prev_inst) *)
-  (*             --> is_entirely_satisfied_load prev_prev_inst)) && *)
-
-  (* (*** Additions for RISCV load-release/store-acquire ***) *)
-  (* (is_RISCV_load_release (ik instruction) --> *)
-  (*     forall (prev_inst MEM inst_context.active_prefix). prev_inst.finished) && *)
-  (* (forall (prev_inst MEM inst_context.active_prefix). *)
-  (*     is_RISCV_store_acquire (ik prev_inst) --> prev_inst.finished) *)
-
-
-
-      Definition try_sat_mem_load_op_from_storage '((MemReadID rid) : mem_read_id)
-        : itree F (list instruction_id) :=
-        s <- get
-        ;; '(_, ins, subts) <- try_get_dec_instruction_state iid s
-        ;; rs <- try_unwrap_option ins.(ins_mem_reads)
-                                        "try_sat_mem_load_op_from_storage: no mem reads."
-        ;; unsat_slcs <- try_unwrap_option (List.nth_error rs.(rs_unsat_slcs) rid)
-                                          "try_sat_mem_load_op_from_storage: missing rid."
-        (* ;; guard (isTrue (unsat_slcs <> [])) *)
-        ;; rr <- try_unwrap_option (List.nth_error rs.(rs_reads) rid)
-                                  "try_sat_mem_load_op_from_storage: missing rid"
-        ;; rf_forward <- try_unwrap_option (List.nth_error rs.(rs_reads_from) rid)
-                                          "try_sat_mem_load_op_from_storage: missing rid."
-        ;; rf_storage <- trigger (StERead rr unsat_slcs)
-        ;; let rs := rs <| rs_unsat_slcs := list_replace_nth rid [] rs.(rs_unsat_slcs) |>
-                        <| rs_reads_from := list_replace_nth rid (rf_forward ++ rf_storage)
-                                                             rs.(rs_reads_from) |> in
-           let ins := ins <| ins_mem_reads := Some rs |> in
-           (* FIXME: compute iids that need to be restarted *)
-           let restarts :=
-               (List.fold_left (fun iids t =>
-                                  List.fold_left (fun iids i =>
-                                                    match i with
-                                                    | inl ins =>
-                                                      if ins.(ins_finished) then iids
-                                                      else ins.(ins_id) :: iids
-                                                    | inr _ => iids
-                                                    end)
-                                                 (tree_to_list_preorder t)
-                                                 iids)
-                               subts
-                               []) in
-           let subts := restart_instructions restarts subts in
-           let s := update_dec_instruction_state_and_subts iid ins subts s in
-           'tt <- put s
-           ;; ret restarts.
-
-      Definition try_complete_load_ops : itree F mem_slc_val :=
-        s <- get
-        ;; '(_, ins, _) <- try_get_dec_instruction_state iid s
-        ;; rs <- try_unwrap_option ins.(ins_mem_reads)
-                                        "try_complete_load_ops: no mem reads."
-        (* ;; guard (isTrue (Forall (fun u => u = []) rs.(rs_unsat_slcs))) *)
-        ;; val <- try_unwrap_option
-                   (mem_slc_val_of_reads_from
-                      rs.(rs_footprint)
-                           (List.concat rs.(rs_reads_from)))
-                   "try_complete_load_ops: some bytes are missing from memory read."
-        ;; ret val.
-
-      Definition try_init_mem_store_op_fps (slc : mem_slc) : itree F unit :=
-        s <- get
-        ;; '(_, ins, _) <- try_get_dec_instruction_state iid s
-        ;; let ws := {| ws_footprint := slc;
-                        ws_writes := [];
-                        ws_has_propagated := [] |} in
-           let ins := ins <| ins_mem_writes := Some ws |> in
-           let s := update_dec_instruction_state iid ins s in
-           put s.
-
-      Definition try_insta_mem_store_op_vals (val : mem_slc_val) : itree F unit :=
-        s <- get
-        ;; '(_, ins, _) <- try_get_dec_instruction_state iid s
-        ;; ws <- try_unwrap_option ins.(ins_mem_writes)
-                                        "try_insta_mem_store_op_vals: no mem writes"
-        ;; let sub_slcs := split_store_mem_slc_val ins.(ins_ast) ws.(ws_footprint) val in
-           let kind := mem_write_kind_of_ast ins.(ins_ast) in
-           let wids := List.seq 0 (List.length sub_slcs) in
-           let writes := List.map
-                           (fun '(wid, (slc, val)) => {| write_id := MemWriteID wid;
-                                                      write_footprint := slc;
-                                                      write_val := val;
-                                                      write_kind := kind |})
-                           (List.combine wids sub_slcs) in
-           let ws := ws <| ws_writes := writes |>
-                                               <| ws_has_propagated := List.map (fun _ => false) writes |>in
-           let ins := ins <| ins_mem_writes := Some ws |> in
-           let s := update_dec_instruction_state iid ins s in
-           put s.
-
-      Definition try_commit_store_instruction : itree F (list mem_write_id) :=
-        s <- get
-        ;; '(_, ins, _) <- try_get_dec_instruction_state iid s
-        ;; ws <- try_unwrap_option ins.(ins_mem_writes)
-                                        "try_commit_store_instruction: no mem writes"
-        (* FIXME: check commit-store condition *)
-        ;; let wids := List.map write_id ws.(ws_writes) in
-           ret wids.
-
-      Definition try_propagate_store_op '((MemWriteID wid) : mem_write_id)
-        : itree F (list instruction_id) :=
-        s <- get
-        ;; '(_, ins, subts) <- try_get_dec_instruction_state iid s
-        ;; ws <- try_unwrap_option ins.(ins_mem_writes)
-                                        "try_propagate_store_op: no mem writes"
-        (* ;; guard (isTrue (List.nth_error ws.(ws_has_propagated) wid = Some false)) *)
-        ;; w <- try_unwrap_option (List.nth_error ws.(ws_writes) wid)
-                                 "try_propagate_store_op: missing wid"
-        (* FIXME: check mem-write-propagation condition *)
-        ;; 'tt <- trigger (StEWrite w)
-        ;; let ws := ws <| ws_has_propagated := list_replace_nth wid true ws.(ws_has_propagated) |> in
-           let ins := ins <| ins_mem_writes := Some ws |> in
-           (* FIXME: compute iids that need to be restarted *)
-           let restarts :=
-               (List.fold_left (fun iids t =>
-                                  List.fold_left (fun iids i =>
-                                                    match i with
-                                                    | inl ins =>
-                                                      if ins.(ins_finished) then iids
-                                                      else ins.(ins_id) :: iids
-                                                    | inr _ => iids
-                                                    end)
-                                                 (tree_to_list_preorder t)
-                                                 iids)
-                               subts
-                               []) in
-           let subts := restart_instructions restarts subts in
-           let s := update_dec_instruction_state_and_subts iid ins subts s in
-           'tt <- put s
-           ;; ret restarts.
-
-      Definition try_complete_store_ops : itree F unit :=
-        (* FIXME: is there anything we need to check here? *)
-        let iid := iid in
-        ret tt.
-
-    End Handle_instruction_instance.
-
-    Definition handle_E {F}
-               `{storageE -< F}
-               `{stateE state -< F}
-               `{exceptE disabled -< F}
-               `{exceptE error -< F}
-               `{debugE -< F}
-               (iid : instruction_id)
-      : E ~> itree F :=
-      fun A e =>
-        let it : itree F A :=
-            match e with
-            | ThEFetchAndDecodeOrRestart => try_fetch_and_decode_or_restart iid
-            | ThEFinishIns => try_finish_instruction iid
-            | ThERegAccess _ e => handle_reg_access iid _ e
-            (* Load events *)
-            | ThEInitMemLoadOps slc => try_init_mem_load_ops iid slc
-            | ThESatMemLoadOpForwarding rid => try_sat_mem_load_op_forwarding iid rid
-            | ThESatMemLoadOpStorage rid => try_sat_mem_load_op_from_storage iid rid
-            | ThECompleteLoadOps => try_complete_load_ops iid
-            (* Store events *)
-            | ThEInitMemStoreOpFps slc => try_init_mem_store_op_fps iid slc
-            | ThEInstaMemStoreOpVals val => try_insta_mem_store_op_vals iid val
-            | ThECommitStoreInstruction => try_commit_store_instruction iid
-            | ThEPropagateStoreOp wid => try_propagate_store_op iid wid
-            | ThECompleteStoreOps => try_complete_store_ops iid
-            end in
-        'tt <- trigger (Debug ("handle_E: " ++ show e))
-        ;; it.
-
-  End State.
+          | ThEFetchAndDecodeOrRestart => try_fetch_and_decode_or_restart iid
+          | ThEFinishIns => try_finish_instruction iid
+          | ThERegAccess _ e => handle_reg_access iid _ e
+          (* Load events *)
+          | ThEInitMemLoadOps slc => try_init_mem_load_ops iid slc
+          | ThESatMemLoadOpForwarding rid => try_sat_mem_load_op_forwarding iid rid
+          | ThESatMemLoadOpStorage rid => try_sat_mem_load_op_from_storage iid rid
+          | ThECompleteLoadOps => try_complete_load_ops iid
+          (* Store events *)
+          | ThEInitMemStoreOpFps slc => try_init_mem_store_op_fps iid slc
+          | ThEInstaMemStoreOpVals val => try_insta_mem_store_op_vals iid val
+          | ThECommitStoreInstruction => try_commit_store_instruction iid
+          | ThEPropagateStoreOp wid => try_propagate_store_op iid wid
+          | ThECompleteStoreOps => try_complete_store_ops iid
+          end in
+      'tt <- trigger (Debug ("handle_E: " ++ show e))
+      ;; it.
 End Make.
